\documentclass[10pt]{article}
\usepackage[utf8]{inputenc}
\usepackage[T1]{fontenc}
\usepackage{amsmath}
\usepackage{amsfonts}
\usepackage{amssymb}
\usepackage[version=4]{mhchem}
\usepackage{stmaryrd}

\begin{document}
Questions.\\
Write about Ornstein-Uhlenbeck (OU) process.\\
Sol-n\\
Consider the General formof Linear SDE (5) from Q1:\\
(1) $d X_{t}=\left[\frac{-a=\text { const }}{\left[a_{1}(t) X_{t}+\stackrel{0}{a_{2}(t)}\right] d t+\left[\begin{array}{l}0 \\ {\left[b_{1}(t) X_{t}+b_{2}(t)\right]}\end{array} d W_{t}\right.}\right.$\\
if\\
(2) $a_{1}(t)=-a=$ cont $, a_{2}(t)=0, b_{1}(t)=0, b_{2}(t)=b=$ const,\\
then we have\\
Ornsfein - Uhlenbeck equation:\\
(3) $d X_{t}=-a X_{t} d t+b d W_{t}$ with the IC:\\
(4) $\quad X_{t}(0)=X_{0}$

Tote (3) is a mon-homogéneur SDE, to we hed integrating factor as follows:\\
(5) $\quad M_{t}=e^{a t}$, then change of variable\\
for (3) is\\
(6) $\quad Y_{t}=X_{t} M_{t}$, so


\begin{equation*}
\varphi\left(X_{t}, t\right)=X_{t} \cdot M_{t}=X_{t} \cdot e^{a t} \tag{1}
\end{equation*}


(7) $\quad \varphi\left(x_{t}, t\right)=x_{t} \cdot e^{a t} \quad$ requires usage of

Ito's formula of case iv:


\begin{align*}
& Y_{t}=\varphi\left(X_{t, t}\right)=X_{t \cdot} e^{a t} \text { with }  \tag{3}\\
& d X_{t}=\underbrace{-a X_{t}}_{\mu_{t}} d t+\underbrace{b}_{\sigma t} d w_{t}
\end{align*}


(8) $d Y_{t}=\left[\frac{\partial \varphi\left(x_{t, t}\right)}{\partial t}+\mu_{t} \frac{\partial \varphi\left(x_{t, t}\right)}{\partial x}+\frac{1}{2} \sigma_{t}^{2} \frac{\partial^{2} \varphi\left(x_{t} t\right)}{\partial x^{2}}\right] d t$

$$
+\sigma_{t} \frac{\partial \varphi\left(x_{t, t}\right)}{\partial x} d W_{t}
$$

so we need\\
$\varphi(x, t)=x \cdot e^{a t}$,\\
$\frac{\partial \varphi(x, t)}{\partial t}=\frac{\partial}{\partial t}\left(x \cdot e^{a t}\right)=a x e^{a t} ;$\\
(9) $\left\{\begin{array}{l}\frac{\partial \varphi(x, t)}{\partial x}=\frac{\partial}{\partial x}\left(x e^{a t}\right)=e^{a t} \\ \frac{\partial \varphi^{2}(x, t)}{\partial x^{2}}=\frac{\partial}{\partial x}\left(e^{a t}\right)=0 ;\end{array}\right.$

Evaluating expressions (a) $x=X_{t}$ in (9) \& plugging back into (8) gives

$$
\begin{aligned}
d Y_{t}=d\left(X_{t} e^{a t}\right) & =\left[a X_{t} e^{a t}+\left(-a X_{t}\right) \cdot e^{a t}+\frac{1}{2} \cdot(t)^{2} \cdot 0\right] d t+ \\
& +(b) \cdot e^{a t} d W_{t} \Rightarrow
\end{aligned}
$$

(10) $d Y_{t}=b e^{a t} d W_{t}$ which can be directly integrated:

$$
\int_{0}^{t} d V_{\tau}=\int_{0}^{t} b e^{a \tau} d w_{\tau} \Rightarrow
$$

(11) $\quad Y_{t}=Y_{0}+\int_{0}^{t} b e^{a \tau} d W_{\tau}$, but by


\begin{equation*}
X_{t} e^{a t}=X_{0} \cdot e_{=1}^{0}+\int_{0}^{t} b e^{a \tau} d W_{\tau} \quad * e^{-a t} o f B S: \tag{3}
\end{equation*}


(12') $X_{t}=X_{0} e^{-a t}+e^{-a t} \cdot \int_{0}^{t} b e^{a \tau} d w_{t}$ or\\
(12) $x_{t}=X_{0} e^{-a t}+\int_{0}^{t} b e^{a(\tau-t)} d w_{\tau}$\\
is the\\
solon for OU eq-n in $(3)+(4)$.\\
(iii) Plotting several statistic paths (wonking with Zach on Wed (Thursday)\\
(iv) Statitics

$$
\begin{aligned}
& E\left[x_{t}\right]=b^{b y(12)} E\left[x_{0} e^{-a t}+\int_{0}^{t} b e^{a(\tau-t)} d W_{\tau}\right] \\
& =E\left[X_{0} e^{-a t}\right]+E\left[\int_{0}^{t} b e^{a(\tau-t)^{0}} d W_{\varepsilon}\right] \\
& E(\#)=\# \text { q } E[\text { Itô Integral }]=0 \\
& =X_{0} e^{-a t} \\
& \text { (13) } E\left[X_{t}\right]=x_{0} e^{-a t}>0 \\
& \operatorname{Var}\left(X_{t}\right)=\operatorname{Var}\left(X_{0} e^{-a t}\right)+\operatorname{Var}\left[\int_{0}^{t} b e^{a(\tau-t)} d w_{c}\right] \\
& =\operatorname{Var}\left[\int_{0}^{t} b e^{a(\tau-t)} d w_{t}\right]= \\
& =E\left[\left(\int_{0}^{t} b e^{a(\tau-t)} d w_{\tau}\right)^{2}\right]-\{[\underbrace{\left[\int_{0}^{t} b_{0}^{a(\tau-t)} d w_{\tau}\right.}_{=0 \text { betry }}]^{2}\}^{2} \\
& \text { Ifio Isometry } \\
& =E\left[\int_{(t)}^{t}\left(b e^{a(\tau-t)}\right)^{2} d \tau\right]=
\end{aligned}
$$

(?1)\\
$=\int_{0}^{t} E\left(b^{2} e^{2 a(\tau-t)}\right) d \tau$\\
$=b^{2} \frac{1-e^{-2 a t}}{2 a}$,\\
i. $e$,\\
(14)

$$
\operatorname{Var}\left(X_{t}\right)=b^{2} \cdot \frac{1-e}{2 a}
$$

rote that os $t \rightarrow \infty$\\
$E\left(X_{t}\right) \rightarrow 0 \quad \& \quad \operatorname{Var}\left(X_{t}\right) \rightarrow \frac{b^{2}}{2 a}=$ const.\\
(15) Auto Corrolation $\left(X_{t}\right)=$

22\\
$\downarrow$\\
How to\\
calculate\\
statisty\\
of GM\\
(4)\\
(15)

$$
\begin{aligned}
& X_{t}=g(t)+b e^{-a t} \cdot Y_{t}, \\
& \operatorname{Cov}\left(X_{t}, X_{s}\right)=\operatorname{cov}\left[b e^{-a t} Y_{t},\left(b e^{-a s}\right) Y_{s}\right] \\
& =b^{2} e^{-a t} \cdot e^{-a s} \operatorname{cov}\left(Y_{t}, Y_{s}\right), \text { and }
\end{aligned}
$$

jo

By (12)\\
$X_{t}=\underbrace{X_{0} e^{-a t}}_{g(t)}+b e^{-a t} \underbrace{\int_{0}^{t} e^{a \tau} d W_{\tau}}_{Y_{t}, 1_{0}}, ~ b t$

WLOG, let $s<t$, ther

$$
\begin{aligned}
& \operatorname{Cov}\left(X_{s}, X_{t}\right)=b^{2} e^{-a(s+t)} \cdot \operatorname{Cov}\left(Y_{s}, Y_{t}\right)_{q} \\
& \operatorname{cov}\left(Y_{p}, Y_{t}\right)=\left[\int_{0}^{3} e^{a \tau} d w_{\tau}, \int_{0}^{t} e^{a \tau} d w_{\tau}\right] \\
& =E\left[Y_{1}, Y_{t}\right]-E\left[Y_{1}\right] \cdot E\left[Y_{t}\right]
\end{aligned}
$$

$$
\begin{aligned}
& -E\left[\int_{0}^{a} e_{0}^{a \tau} d w_{\tau}\right] \cdot E\left[\int_{0}^{0} e^{a \tau} d w_{\tau}\right]
\end{aligned}
$$

a) $\quad 1<t$

$$
\begin{aligned}
& \left.=E\left[\int_{0}^{1} e^{a \tau} d w_{\tau} \cdot \int_{0}^{1} e^{a \tau} d w_{\tau}+\int_{1}^{t} e^{a \tau} d w_{\tau}\right]\right]-0 \\
& =E\left[\left(\int_{0}^{1} e^{a \tau} \frac{d w_{\tau}}{=d \tau}\right)^{2}\right]+E\left[\int_{0}^{1} e^{a \tau} d w_{\tau} \cdot \int_{0}^{t} e^{a \tau} d w_{\tau}\right] \\
& =E\left[\int_{0}^{1} e^{2 a \tau} d \tau\right]+0 \quad(? 3) w h y \\
& =\frac{e^{2 a}}{2 a}\left[\left.e^{\tau}\right|_{\tau=1} ^{\tau=1}\right]=\frac{e^{2 a}}{2 a} \cdot\left[e^{p}-1\right] \cdot S_{0}
\end{aligned}
$$

Itô\\
(17) $\operatorname{Cov}\left(Y_{f}, Y_{t}\right)=\frac{e^{2 a}}{2 a}\left[e^{s}-1\right]$.

Pluggiy (17) back to (16):

$$
\begin{aligned}
\operatorname{Cov}\left(X_{1}, X_{t}\right) & =b^{2} e^{-a(1+t)} \cdot \operatorname{Cov}\left(Y_{1}, Y_{t}\right) \\
& =b^{2} \cdot e^{-a(1+t)} \cdot e^{2 a}\left[e^{1}-1\right] \\
& =\frac{b^{2}}{2 a} e^{a(-1-t+2)^{2 a}} \cdot\left[e^{1}-1\right], \Rightarrow
\end{aligned}
$$

(18)\\
(7) assuming $s<t$.\\
in General, presentiy with min $\{1, t\}$ :\\
(19) $\operatorname{Cov}\left(X_{1}, X_{t}\right)=b^{2} \cdot e^{a(-1-t+2} \cdot\left[e^{\sin \{1, t\}}-1\right]$

Note as $f \rightarrow \infty$\\
(2d) $\operatorname{Cov}\left(X_{3}, X_{t}\right)=\frac{b^{2}}{2 a} e^{|t-1|}$\\
a) devired.\\
(8)


\end{document}